code/hash-new/Hacl.SHA1.fst
@@ -1,0 +1,97 @@
+module Hacl.SHA1
+
+include Hacl.Hash.Common
+open Spec.Hash.Helpers
+
+module B = LowStar.Buffer
+module IB = LowStar.ImmutableBuffer
+module HS = FStar.HyperStack
+module HST = FStar.HyperStack.ST
+module Spec = Spec.SHA1
+module U8 = FStar.UInt8
+module U32 = FStar.UInt32
+module E = FStar.Kremlin.Endianness
+module CE = C.Endianness
+
+friend Spec.SHA1
+
+(** Top-level constant arrays for the MD5 algorithm. *)
+let h0 = IB.igcmalloc_of_list HS.root Spec.init_as_list
+
+
+let alloca () =
+  B.alloca_of_list Spec.init_as_list
+
+let static_fp () =
+  B.loc_addr_of_buffer h0
+
+let recall_static_fp () =
+  B.recall h0
+
+let init s =
+  IB.recall_contents h0 (Seq.seq_of_list Spec.init_as_list);
+  B.blit h0 0ul s 0ul 5ul
+
+let working_state_matches (h: HS.mem) (w: Spec.working_state) (s: state SHA1) : GTot Type0 =
+  let s' = B.as_seq h s in
+  w.Spec.a == Seq.index s' 0 /\
+  w.Spec.b == Seq.index s' 1 /\
+  w.Spec.c == Seq.index s' 2 /\
+  w.Spec.d == Seq.index s' 3 /\
+  w.Spec.e == Seq.index s' 4
+
+inline_for_extraction
+let w_t = (b: B.lbuffer (word SHA1) 80)
+
+inline_for_extraction
+let block_t = (block: B.buffer U8.t { B.length block == size_block SHA1 } )
+
+let w_inv (h0: HS.mem) (h: HS.mem) (m: block_t) (b: w_t) (i: nat) : GTot Type0 =
+  B.disjoint m b /\
+  B.live h0 m /\
+  B.live h m /\
+  B.live h b /\
+  B.modifies (B.loc_buffer b) h0 h /\ (
+    let mi = E.seq_uint32_of_be size_block_w (B.as_seq h0 m) in
+    let s = B.as_seq h b in
+    (forall (j: nat) . (j < i /\ j < 80) ==> Spec.w mi (U32.uint_to_t j) == Seq.index s j)
+  )
+
+inline_for_extraction
+let index_32_be' (n: Ghost.erased nat) (b: B.buffer UInt8.t) (i: UInt32.t):
+  HST.Stack UInt32.t
+    (requires (fun h ->
+      B.live h b /\ B.length b == 4 `Prims.op_Multiply` Ghost.reveal n /\
+      UInt32.v i < Ghost.reveal n))
+    (ensures (fun h0 r h1 ->
+      B.(modifies loc_none h0 h1) /\
+      r = Seq.index (E.seq_uint32_of_be (Ghost.reveal n) (B.as_seq h0 b)) (UInt32.v i)))
+= CE.index_32_be b i
+
+inline_for_extraction
+let w_body_value (h0: HS.mem) (m: block_t) (b: w_t) (i: U32.t) : HST.Stack U32.t
+  (requires (fun h -> w_inv h0 h m b (U32.v i) /\ U32.v i < 80))
+  (ensures (fun h v h' -> B.modifies B.loc_none h h' /\ v == Spec.w (E.seq_uint32_of_be size_block_w (B.as_seq h0 m)) i))
+= if U32.lt i 16ul
+  then
+    index_32_be' (Ghost.hide size_block_w) m i
+  else
+    let wmit3 = B.index b (i `U32.sub` 3ul) in
+    let wmit8 = B.index b (i `U32.sub` 8ul) in
+    let wmit14 = B.index b (i `U32.sub` 14ul) in
+    let wmit16 = B.index b (i `U32.sub` 16ul) in
+    Spec.rotl 1ul (wmit3 `U32.logxor` wmit8 `U32.logxor` wmit14 `U32.logxor` wmit16)
+
+(*
+let w_body (h0: HS.mem) (m: block_t) (b: w_t) (i: U32.t) : HST.Stack unit
+  (requires (fun h -> w_inv h0 h m b (U32.v i) /\ U32.v i < 80))
+  (ensures (fun _ _ h' -> w_inv h0 h' m b (U32.v i + 1)))
+= if U32.lt i 16ul
+  then B.upd b i (CE.index_32_be m i)
+  else
+    let wmit3 = B.index b (i `U32.sub` 3ul) in
+    let wmit8 = B.index b (i `U32.sub` 8ul) in
+    let wmit14 = B.index b (i `U32.sub` 14ul) in
+    let wmit16 = B.index b (i `U32.sub` 16ul) in
+    let v = Spec.rotl 1ul (wmit3 `U32.logxor` wmit8 `U32.logxor` wmit14 `U32.logxor` wmit16) in
+    B.upd b i v
