code/hash-new/Hacl.SHA1.fsti
@@ -1,0 +1,52 @@
+module Hacl.SHA1
+
+include Hacl.Hash.Common
+open Spec.Hash.Helpers
+
+module U8 = FStar.UInt8
+module B = LowStar.Buffer
+module HS = FStar.HyperStack
+module HST = FStar.HyperStack.ST
+module Spec = Spec.SHA1
+
+val alloca: unit -> HST.StackInline (state SHA1)
+  (requires (fun h ->
+    HS.is_stack_region (HS.get_tip h)))
+  (ensures (fun h0 s h1 ->
+    B.(modifies B.loc_none h0 h1) /\
+    B.live h1 s /\
+    B.as_seq h1 s = Spec.init))
+
+val static_fp: unit -> GTot B.loc
+
+let loc_in (l: B.loc) (h: HS.mem) =
+  B.(loc_not_unused_in h `loc_includes` l)
+
+(* A useful lemma for clients, to be called at any time before performing an
+   allocation, hence giving them "for free" that their allocation is disjoint from
+   our top-level arrays. *)
+val recall_static_fp: unit -> HST.Stack unit
+  (requires (fun _ -> True))
+  (ensures (fun h0 _ h1 ->
+    B.(modifies loc_none h0 h1) /\
+    static_fp () `loc_in` h1))
+
+val init (s: state SHA1) : HST.Stack unit
+  (requires (fun h ->
+    B.loc_disjoint (B.loc_addr_of_buffer s) (static_fp ()) /\
+    B.live h s))
+  (ensures (fun h0 _ h1 ->
+    B.(modifies (loc_buffer s) h0 h1) /\
+    Seq.equal (B.as_seq h1 s) Spec.init))
+
+val update
+  (s:state SHA1)
+  (block:B.buffer U8.t { B.length block = size_block SHA1 })
+: HST.Stack unit
+    (requires (fun h ->
+      B.loc_disjoint (B.loc_union (B.loc_buffer s) (B.loc_buffer block)) (static_fp ()) /\
+      B.live h s /\ B.live h block /\ B.disjoint s block))
+    (ensures (fun h0 _ h1 ->
+      B.(modifies (loc_buffer s) h0 h1) /\
+      B.live h1 s /\
+      B.as_seq h1 s == Spec.update (B.as_seq h0 s) (B.as_seq h0 block)))
